coq_translation/examples-from-rust-book/custom_types/enums_testcase_linked_list.v
@@ -10,13 +10,13 @@ Module ImplList.
   Definition prepend (self : List) (elem : u32) : List :=
     Cons elem (ImplBox.new self).
   
-  Definition len (self : static_ref List) : u32 :=
+  Definition len (self : ref List) : u32 :=
     match deref self with
     | Cons (_, tail) => add 1 (len tail)
     | Nil => 0
     end.
   
-  Definition stringify (self : static_ref List) : String :=
+  Definition stringify (self : ref List) : String :=
     match deref self with
     | Cons (head, tail) =>
       let res :=
