coq_translation/examples-from-rust-book/error_handling/other_uses_of_question_mark.v
@@ -3,15 +3,15 @@ Require Import CoqOfRust.CoqOfRust.
 
 Error TyAlias.
 
-Error Struct.
+Error StructUnit.
 
 Module Impl__crate_fmt_Debug_for_EmptyVec.
   Definition Self := EmptyVec.
   
-  #[global] Instance I : _crate.fmt.Debug.Class Self := {|
-    fmt
-      (self : static_ref EmptyVec)
-      (f : mut_ref _crate.fmt.Formatter) :=
+  Global Instance I : _crate.fmt.Debug.Class Self := {|
+    _crate.fmt.Debug.fmt
+        (self : ref EmptyVec)
+        (f : mut_ref _crate.fmt.Formatter) :=
       _crate::fmt::ImplFormatter.write_str f "EmptyVec";
   |}.
 Module ImplEmptyVec.
@@ -19,10 +19,8 @@ Module ImplEmptyVec.
 Module Impl_fmt_Display_for_EmptyVec.
   Definition Self := EmptyVec.
   
-  #[global] Instance I : fmt.Display.Class Self := {|
-    fmt
-      (self : static_ref EmptyVec)
-      (f : mut_ref fmt.Formatter) :=
+  Global Instance I : fmt.Display.Class Self := {|
+    fmt.Display.fmt (self : ref EmptyVec) (f : mut_ref fmt.Formatter) :=
       write_fmt
         f
         (_crate::fmt::ImplArguments.new_v1 ["invalid first item to double"] []);
@@ -32,8 +30,7 @@ Module ImplEmptyVec.
 Module Impl_error_Error_for_EmptyVec.
   Definition Self := EmptyVec.
   
-  #[global] Instance I : error.Error.Class Self := {|
-  |}.
+  Global Instance I : error.Error.Class Self := error.Error.Build_Class _.
 Module ImplEmptyVec.
 
 Definition double_first (_ : unit) :=
