coq_translation/examples-from-rust-book/error_handling/wrapping_errors.v
@@ -8,10 +8,10 @@ Error Enum.
 Module Impl__crate_fmt_Debug_for_DoubleError.
   Definition Self := DoubleError.
   
-  #[global] Instance I : _crate.fmt.Debug.Class Self := {|
-    fmt
-      (self : static_ref DoubleError)
-      (f : mut_ref _crate.fmt.Formatter) :=
+  Global Instance I : _crate.fmt.Debug.Class Self := {|
+    _crate.fmt.Debug.fmt
+        (self : ref DoubleError)
+        (f : mut_ref _crate.fmt.Formatter) :=
       match self with
       | DoubleError.EmptyVec =>
         _crate::fmt::ImplFormatter.write_str f "EmptyVec"
@@ -24,10 +24,8 @@ Module ImplDoubleError.
 Module Impl_fmt_Display_for_DoubleError.
   Definition Self := DoubleError.
   
-  #[global] Instance I : fmt.Display.Class Self := {|
-    fmt
-      (self : static_ref DoubleError)
-      (f : mut_ref fmt.Formatter) :=
+  Global Instance I : fmt.Display.Class Self := {|
+    fmt.Display.fmt (self : ref DoubleError) (f : mut_ref fmt.Formatter) :=
       match deref self with
       | DoubleError.EmptyVec =>
         write_fmt
@@ -48,9 +46,8 @@ Module ImplDoubleError.
 Module Impl_error_Error_for_DoubleError.
   Definition Self := DoubleError.
   
-  #[global] Instance I : error.Error.Class Self := {|
-    source
-      (self : static_ref DoubleError) :=
+  Global Instance I : error.Error.Class Self := {|
+    error.Error.source (self : ref DoubleError) :=
       match deref self with
       | DoubleError.EmptyVec => None
       | DoubleError.Parse (e) => Some e
@@ -61,8 +58,8 @@ Module ImplDoubleError.
 Module Impl_From_for_DoubleError.
   Definition Self := DoubleError.
   
-  #[global] Instance I : From.Class Self := {|
-    from (err : ParseIntError) := DoubleError.Parse err;
+  Global Instance I : From.Class Self := {|
+    From.from (err : ParseIntError) := DoubleError.Parse err;
   |}.
 Module ImplDoubleError.
 
