coq_translation/examples-from-rust-book/scoping_rules/scoping_rules_borrowing_the_ref_pattern.v
@@ -12,9 +12,8 @@ Definition Point : Set := Point.t.
 Module Impl__crate_clone_Clone_for_Point.
   Definition Self := Point.
   
-  #[global] Instance I : _crate.clone.Clone.Class Self := {|
-    clone
-      (self : static_ref Point) :=
+  Global Instance I : _crate.clone.Clone.Class Self := {|
+    _crate.clone.Clone.clone (self : ref Point) :=
       let _ := tt in
       deref self;
   |}.
@@ -23,8 +22,8 @@ Module ImplPoint.
 Module Impl__crate_marker_Copy_for_Point.
   Definition Self := Point.
   
-  #[global] Instance I : _crate.marker.Copy.Class Self := {|
-  |}.
+  Global Instance I : _crate.marker.Copy.Class Self :=
+      _crate.marker.Copy.Build_Class _.
 Module ImplPoint.
 
 Definition main (_ : unit) :=
