coq_translation/examples-from-rust-book/scoping_rules/scoping_rules_lifetimes_traits.v
@@ -3,7 +3,7 @@ Require Import CoqOfRust.CoqOfRust.
 
 Module Borrowed.
   Record t : Set := {
-    x : static_ref i32;
+    x : ref i32;
   }.
 End Borrowed.
 Definition Borrowed : Set := Borrowed.t.
@@ -11,10 +11,10 @@ Definition Borrowed : Set := Borrowed.t.
 Module Impl__crate_fmt_Debug_for_Borrowed.
   Definition Self := Borrowed.
   
-  #[global] Instance I : _crate.fmt.Debug.Class Self := {|
-    fmt
-      (self : static_ref Borrowed<'a>)
-      (f : mut_ref _crate.fmt.Formatter) :=
+  Global Instance I : _crate.fmt.Debug.Class Self := {|
+    _crate.fmt.Debug.fmt
+        (self : ref Borrowed<'a>)
+        (f : mut_ref _crate.fmt.Formatter) :=
       _crate::fmt::ImplFormatter.debug_struct_field1_finish
         f
         "Borrowed"
@@ -26,8 +26,8 @@ Module ImplBorrowed.
 Module Impl_Default_for_Borrowed.
   Definition Self := Borrowed.
   
-  #[global] Instance I : Default.Class Self := {|
-    default  := {| Self.x := 10; |};
+  Global Instance I : Default.Class Self := {|
+    Default.default  := {| Self.x := 10; |};
   |}.
 Module ImplBorrowed.
 
