coq_translation/examples-from-rust-book/scoping_rules/scoping_rules_ownership_and_rules_partial_moves.v
@@ -14,10 +14,10 @@ Definition Person : Set := Person.t.
 Module Impl__crate_fmt_Debug_for_Person.
   Definition Self := Person.
   
-  #[global] Instance I : _crate.fmt.Debug.Class Self := {|
-    fmt
-      (self : static_ref main::Person)
-      (f : mut_ref _crate.fmt.Formatter) :=
+  Global Instance I : _crate.fmt.Debug.Class Self := {|
+    _crate.fmt.Debug.fmt
+        (self : ref main::Person)
+        (f : mut_ref _crate.fmt.Formatter) :=
       _crate::fmt::ImplFormatter.debug_struct_field2_finish
         f
         "Person"
